
***

# Simplification Aptitude Quiz

### **Question 1**
Simplify: `(957 + 932)² - 4 x 957 x 932`

**Correct Answer:** 625

**Solution Explanation:**
This expression matches the algebraic identity $(a+b)² - 4ab$.
-   We know that $(a+b)² - 4ab = (a² + 2ab + b²) - 4ab = a² - 2ab + b² = (a-b)²$.
-   Here, let **a = 957** and **b = 932**.
-   The expression becomes $(957 - 932)²$.
-   $(25)² = \textbf{625}$.

---

### **Question 2**
Simplify: `9 / [5 + 7 / {9+9 / (9 + 9 / 4)}]`

**Correct Answer:** 63/40

**Solution Explanation:**
We solve this by working from the innermost bracket outwards, following the BODMAS rule.
1.  Innermost bracket: $9 + 9/4 = 36/4 + 9/4 = 45/4$.
2.  Next level (division): $9 / (45/4) = 9 \times 4/45 = 36/45 = 4/5$.
3.  Curly braces: $9 + 4/5 = 45/5 + 4/5 = 49/5$.
4.  Next level (division): $7 / (49/5) = 7 \times 5/49 = 35/49 = 5/7$.
5.  Square brackets: $5 + 5/7 = 35/7 + 5/7 = 40/7$.
6.  Final division: $9 / (40/7) = 9 \times 7/40 = \textbf{63/40}$.

---

### **Question 3**
Simplify: `983² - 17²`

**Correct Answer:** 966,000

**Solution Explanation:**
This expression is in the form of the algebraic identity $a² - b²$.
-   We know that $a² - b² = (a - b)(a + b)$.
-   Here, let **a = 983** and **b = 17**.
-   The expression becomes $(983 - 17)(983 + 17)$.
-   $(966)(1000) = \textbf{966,000}$.

---

### **Question 4**
What is the value of `11 / [ 1 + 1 / { 1 + 1 / ( 1 + 1/ 3 ) } ]`?

**Correct Answer:** 7

**Solution Explanation:**
This is a continued fraction. We solve it from the bottom up.
1.  Innermost part: $1 + 1/3 = 4/3$.
2.  Next level: $1 / (4/3) = 3/4$.
3.  Next level: $1 + 3/4 = 7/4$.
4.  Next level: $1 / (7/4) = 4/7$.
5.  Final denominator: $1 + 4/7 = 11/7$.
6.  Final expression: $11 / (11/7) = 11 \times 7/11 = \textbf{7}$.

---

### **Question 5**
Simplify: `24 - [52 - {4 + 10 x (-3)}]`

**Correct Answer:** -54

**Solution Explanation:**
We solve using the BODMAS rule (Brackets, Orders, Division, Multiplication, Addition, Subtraction).
1.  Innermost braces `{}`: First, multiply `10 x (-3) = -30`. Then add `4 + (-30) = -26`.
2.  Square brackets `[]`: `52 - {-26}` becomes `52 + 26 = 78`.
3.  Final calculation: `24 - 78 =` **-54**.

---

### **Question 6**
Simplify: `((82 x 82) - ( 18 x 18))¹/²`

**Correct Answer:** 80

**Solution Explanation:**
The expression can be written as `(82² - 18²)¹/²` or `√(82² - 18²)`.
-   We use the identity $a² - b² = (a - b)(a + b)$.
-   `√((82 - 18)(82 + 18))`
-   `√((64)(100))`
-   `√6400 =` **80**.

---

### **Question 7**
What is the value of `( 1 1/4 ÷ 2 3/5 ) ÷ 1 7/13`?

**Correct Answer:** 5/16

**Solution Explanation:**
1.  Convert all mixed fractions to improper fractions:
    -   $1\ 1/4 = 5/4$
    -   $2\ 3/5 = 13/5$
    -   $1\ 7/13 = 20/13$
2.  Solve the part in the parenthesis first:
    -   $5/4 ÷ 13/5 = 5/4 \times 5/13 = 25/52$.
3.  Perform the final division:
    -   $25/52 ÷ 20/13 = 25/52 \times 13/20$.
    -   Simplify: $\frac{25}{20} \times \frac{13}{52} = \frac{5}{4} \times \frac{1}{4} = \textbf{5/16}$.

---

### **Question 8**
Simplify `p³ + 27`.

**Correct Answer:** `(p + 3)(p² - 3p + 9)`

**Solution Explanation:**
This is in the form of the sum of cubes identity: $a³ + b³ = (a + b)(a² - ab + b²)$.
-   Here, **a = p** and **b = 3** (since $3³ = 27$).
-   Substituting into the formula gives: `(p + 3)(p² - (p)(3) + 3²)`.
-   This simplifies to **`(p + 3)(p² - 3p + 9)`**.

---

### **Question 9**
If `2945 / 19 - 11 x 5 = 29 + a`, find the value of `a`.

**Correct Answer:** 71

**Solution Explanation:**
First, simplify the left-hand side (LHS) using BODMAS.
1.  Division: `2945 / 19 = 155`.
2.  Multiplication: `11 x 5 = 55`.
3.  Subtraction: `155 - 55 = 100`.
4.  So the equation is `100 = 29 + a`.
5.  Solve for a: `a = 100 - 29 =` **71**.

---

### **Question 10**
What is the value of `(4³ + 4) / [5² - (7² - 41)]`?

**Correct Answer:** 4

**Solution Explanation:**
1.  Simplify the numerator: $4³ + 4 = 64 + 4 = 68$.
2.  Simplify the denominator:
    -   Innermost bracket: $7² - 41 = 49 - 41 = 8$.
    -   Main denominator: $5² - 8 = 25 - 8 = 17$.
3.  Perform the final division: $68 / 17 = \textbf{4}$.

---
---

### **Question 11**
Simplify: `(87 x 87 + 61 x 61 - 2 x 87 x 61)`

**Correct Answer:** 676

**Solution Explanation:**
This expression matches the algebraic identity $a² + b² - 2ab$.
-   We know that $a² + b² - 2ab = (a - b)²$.
-   Here, let **a = 87** and **b = 61**.
-   The expression becomes $(87 - 61)²$.
-   $(26)² = \textbf{676}$.

---

### **Question 12**
Simplify: `3 1/3 ÷ 6 3/7 of 1 1/4`

**Correct Answer:** 56/135

**Solution Explanation:**
According to BODMAS, 'of' is calculated before 'division'.
1.  Convert to improper fractions: $10/3 ÷ 45/7$ of $5/4$.
2.  Calculate the 'of' part first: $45/7 \times 5/4 = 225/28$.
3.  Now the expression is: $10/3 ÷ 225/28$.
4.  Perform the division: $10/3 \times 28/225$.
5.  Simplify: $\frac{10}{225} \times \frac{28}{3} = \frac{2}{45} \times \frac{28}{3} = \textbf{56/135}$.

---

### **Question 13**
If `x/y = 6/5`, find the value of `(x² + y²) / (x² - y²)`.

**Correct Answer:** 61/11

**Solution Explanation:**
1.  Divide the numerator and the denominator of the expression by `y²`:
    -   $\frac{(x²/y²) + (y²/y²)}{(x²/y²) - (y²/y²)} = \frac{(x/y)² + 1}{(x/y)² - 1}$
2.  Substitute the given value `x/y = 6/5` into the new expression:
    -   $\frac{(6/5)² + 1}{(6/5)² - 1} = \frac{(36/25) + 1}{(36/25) - 1}$
3.  Simplify the numerator and denominator:
    -   Numerator: $36/25 + 25/25 = 61/25$.
    -   Denominator: $36/25 - 25/25 = 11/25$.
4.  Perform the final division: $(61/25) / (11/25) = 61/25 \times 25/11 = \textbf{61/11}$.

---

### **Question 14**
Simplify: `(10² + 11² + 12²) / (13² - 160)`

**Correct Answer:** 365/9

**Solution Explanation:**
1.  Simplify the numerator: $100 + 121 + 144 = 365$.
2.  Simplify the denominator: $169 - 160 = 9$.
3.  The final simplified fraction is **365/9**.

---

### **Question 15**
Find the value of `√72 + √72 + √72 + ...` up to infinity.

**Correct Answer:** 9

**Solution Explanation:**
This is an infinite nested radical problem.
1.  Let `x = √72 + √72 + √72 + ...`
2.  Since the expression is infinite, we can write: `x = √(72 + x)`.
3.  Square both sides to remove the radical: `x² = 72 + x`.
4.  Rearrange into a quadratic equation: `x² - x - 72 = 0`.
5.  Factor the quadratic equation. We need two numbers that multiply to -72 and add to -1. These numbers are -9 and +8.
    -   `(x - 9)(x + 8) = 0`.
6.  The possible values for x are 9 and -8. Since the square root of a positive number cannot be negative, we discard -8.
7.  Therefore, `x =` **9**.
